coq/NNRSimp/Lang/NNRSimpRename.v
@@ -1,0 +1,809 @@
+(*
+ * Copyright 2015-2016 IBM Corporation
+ *
+ * Licensed under the Apache License, Version 2.0 (the "License");
+ * you may not use this file except in compliance with the License.
+ * You may obtain a copy of the License at
+ *
+ * http://www.apache.org/licenses/LICENSE-2.0
+ *
+ * Unless required by applicable law or agreed to in writing, software
+ * distributed under the License is distributed on an "AS IS" BASIS,
+ * WITHOUT WARRANTIES OR CONDITIONS OF ANY KIND, either express or implied.
+ * See the License for the specific language governing permissions and
+ * limitations under the License.
+ *)
+
+Require Import String.
+Require Import List.
+Require Import Arith.
+Require Import EquivDec.
+Require Import Morphisms.
+Require Import Arith.
+Require Import Max.
+Require Import Bool.
+Require Import Peano_dec.
+Require Import EquivDec.
+Require Import Decidable.
+Require Import Utils.
+Require Import CommonRuntime.
+Require Import NNRSimp.
+Require Import NNRSimpVars.
+Require Import NNRSimpUsage.
+Require Import NNRSimpEval.
+
+Section NNRSimpRename.
+
+  Context {fruntime:foreign_runtime}.
+
+  Fixpoint nnrs_imp_expr_rename (e:nnrs_imp_expr) (from to:var) : nnrs_imp_expr
+    := match e with 
+       | NNRSimpGetConstant c =>
+         NNRSimpGetConstant c
+       | NNRSimpVar v =>
+         NNRSimpVar (if v == from then to else v)
+       | NNRSimpConst d =>
+         NNRSimpConst d
+       | NNRSimpBinop b e₁ e₂ =>
+         NNRSimpBinop b
+                      (nnrs_imp_expr_rename e₁ from to)
+                      (nnrs_imp_expr_rename e₂ from to)
+       | NNRSimpUnop u e₁ =>
+         NNRSimpUnop u
+                     (nnrs_imp_expr_rename e₁ from to)
+       | NNRSimpGroupBy g sl e₁ =>
+         NNRSimpGroupBy g sl
+                        (nnrs_imp_expr_rename e₁ from to)
+       end.
+
+  Fixpoint nnrs_imp_stmt_rename (s:nnrs_imp_stmt) (from to:var) : nnrs_imp_stmt
+    := match s with
+       | NNRSimpSkip =>
+         NNRSimpSkip
+       | NNRSimpSeq s₁ s₂ =>
+         NNRSimpSeq
+           (nnrs_imp_stmt_rename s₁ from to)
+           (nnrs_imp_stmt_rename s₂ from to)
+       | NNRSimpAssign v e =>
+         NNRSimpAssign
+           (if v == from then to else v)
+           (nnrs_imp_expr_rename e from to)
+       | NNRSimpLet v eo s₀ =>
+         NNRSimpLet v 
+                    (match eo with
+                     | None => None
+                     | Some e => Some (nnrs_imp_expr_rename e from to)
+                     end)
+                    (if v == from
+                     then s₀
+                     else nnrs_imp_stmt_rename s₀ from to)
+       | NNRSimpFor v e s₀ =>
+         NNRSimpFor v
+                    (nnrs_imp_expr_rename e from to)
+                    (if v == from
+                     then s₀
+                     else nnrs_imp_stmt_rename s₀ from to)
+       | NNRSimpIf e s₁ s₂ =>
+         NNRSimpIf
+           (nnrs_imp_expr_rename e from to)
+           (nnrs_imp_stmt_rename s₁ from to)
+           (nnrs_imp_stmt_rename s₂ from to)
+       | NNRSimpEither e x₁ s₁ x₂ s₂ =>
+         NNRSimpEither
+           (nnrs_imp_expr_rename e from to)
+           x₁
+           (if x₁ == from
+            then s₁
+            else nnrs_imp_stmt_rename s₁ from to)
+           x₂
+           (if x₂ == from
+            then s₂
+            else nnrs_imp_stmt_rename s₂ from to)
+       end.
+
+  Section vars.
+
+    Lemma nnrs_imp_stmt_rename_bound_vars
+          (s:nnrs_imp_stmt) (from to:var) :
+      nnrs_imp_stmt_bound_vars (nnrs_imp_stmt_rename s from to)
+      = nnrs_imp_stmt_bound_vars s.
+    Proof.
+      induction s; simpl; try congruence
+      ; repeat (match_destr; try congruence).
+    Qed.
+    
+    Lemma nnrs_imp_expr_rename_free_vars
+          (e:nnrs_imp_expr) (from to:var) :
+      nnrs_imp_expr_free_vars (nnrs_imp_expr_rename e from to)
+      = replace_all (nnrs_imp_expr_free_vars e) from to.
+    Proof.
+      induction e; simpl; trivial.
+      rewrite IHe1, IHe2, replace_all_app; trivial.
+    Qed.
+
+    Lemma nnrs_imp_stmt_rename_free_vars
+          (s:nnrs_imp_stmt) (from to:var) :
+      ~ In to (nnrs_imp_stmt_bound_vars s) ->
+      nnrs_imp_stmt_free_vars (nnrs_imp_stmt_rename s from to)
+      = replace_all (nnrs_imp_stmt_free_vars s) from to.
+    Proof.
+      induction s; simpl; repeat rewrite in_app_iff; intros inn; trivial
+      ; repeat rewrite nnrs_imp_expr_rename_free_vars
+      ; repeat rewrite replace_all_app
+      ; simpl; trivial
+      ; string_eqdec_to_equiv.
+      - rewrite IHs1, IHs2 by tauto; trivial.
+      - destruct o; simpl.
+        + rewrite nnrs_imp_expr_rename_free_vars.
+          f_equal.
+          match_destr; unfold equiv, complement in *.
+          * subst.
+            rewrite replace_all_remove_eq; trivial.
+          * rewrite IHs by tauto.
+            rewrite remove_replace_all_comm by tauto.
+            trivial.
+        + match_destr; unfold equiv, complement in *.
+          * subst.
+            rewrite replace_all_remove_eq; trivial.
+          * rewrite IHs by tauto.
+            rewrite remove_replace_all_comm by tauto.
+            trivial.
+      - f_equal.
+        match_destr; unfold equiv, complement in *.
+        + subst.
+          rewrite replace_all_remove_eq; trivial.
+        + rewrite IHs by tauto.
+          rewrite remove_replace_all_comm by tauto.
+          trivial.
+      - rewrite IHs1, IHs2 by tauto; trivial.
+      - f_equal.
+        f_equal.
+        + match_destr; unfold equiv, complement in *.
+          * subst.
+            rewrite replace_all_remove_eq; trivial.
+          * rewrite IHs1 by tauto.
+            rewrite remove_replace_all_comm by tauto.
+            trivial.
+        + match_destr; unfold equiv, complement in *.
+          * subst.
+            rewrite replace_all_remove_eq; trivial.
+          * simpl in *. rewrite IHs2 by tauto.
+            rewrite remove_replace_all_comm by tauto.
+            trivial.
+    Qed.
+
+  End vars.
+
+  Section var_usage.
+
+    Lemma nnrs_imp_expr_rename_may_use_neq e v v' v0 :
+      v0 <> v ->
+      v0 <> v' ->
+      nnrs_imp_expr_may_use (nnrs_imp_expr_rename e v v') v0 =
+      nnrs_imp_expr_may_use e v0.
+    Proof.
+      induction e; simpl; intros
+      ; repeat rewrite IHe by tauto
+      ; repeat rewrite IHe1 by tauto
+      ; repeat rewrite IHe2 by tauto
+      ; trivial.
+      match_destr.
+      unfold equiv_decb in *.
+      repeat match_destr; congruence.
+    Qed.
+
+    Lemma nnrs_imp_stmt_rename_var_usage_neq s v v' v0 :
+      v0 <> v ->
+      v0 <> v' ->
+      nnrs_imp_stmt_var_usage (nnrs_imp_stmt_rename s v v') v0 =
+      nnrs_imp_stmt_var_usage s v0.
+    Proof.
+      nnrs_imp_stmt_cases (induction s) Case; simpl; intros
+      ; repeat rewrite nnrs_imp_expr_rename_may_use_neq
+      ; repeat rewrite IHs by tauto
+      ; repeat rewrite IHs1 by tauto
+      ; repeat rewrite IHs2 by tauto
+      ; trivial.
+      - Case "NNRSimpAssign"%string.
+        match_destr.
+        unfold equiv_decb.
+        destruct (equiv_dec v1 v)
+        ; destruct (equiv_dec v1 v0)
+        ; destruct (equiv_dec v' v0)
+        ; try congruence.
+      - Case "NNRSimpLet"%string.
+        destruct o
+        ; repeat rewrite nnrs_imp_expr_rename_may_use_neq
+        ; repeat rewrite IHs by tauto
+        ; repeat match_destr; eauto.
+      - Case "NNRSimpFor"%string.
+        match_destr.
+        unfold equiv_decb.
+        destruct (equiv_dec v1 v0); trivial.
+        destruct (equiv_dec v1 v); trivial.
+        rewrite IHs; tauto.
+      - Case "NNRSimpEither"%string.
+        match_destr.
+        destruct (v1 == v0)
+        ; destruct (v2 == v0)
+        ; trivial
+        ; destruct (v1 == v)
+        ; destruct (v2 == v)
+        ; trivial
+        ; repeat rewrite IHs1 by tauto
+        ; repeat rewrite IHs2 by tauto
+        ; trivial.
+    Qed.
+
+  End var_usage.
+
+  Section id.
+    
+    Lemma nnrs_imp_expr_rename_id
+          (e:nnrs_imp_expr) (v:var) :
+      nnrs_imp_expr_rename e v v = e.
+    Proof.
+      induction e; simpl; try congruence.
+      match_destr; congruence.
+    Qed.
+
+    Lemma nnrs_imp_stmt_rename_id
+          (s:nnrs_imp_stmt) (v:var) :
+      nnrs_imp_stmt_rename s v v = s.
+    Proof.
+      induction s; simpl
+      ; repeat rewrite nnrs_imp_expr_rename_id
+      ; try congruence
+      ; repeat (match_destr
+                ; repeat rewrite nnrs_imp_expr_rename_id 
+                ; try congruence).
+    Qed.
+
+  End id.
+
+  Section nfree.
+    
+    Lemma nnrs_imp_expr_rename_nin e from to :
+      ~ In from (nnrs_imp_expr_free_vars e) ->
+      nnrs_imp_expr_rename e from to = e.
+    Proof.
+      induction e; simpl
+      ; repeat rewrite in_app_iff
+      ; intros
+      ; try congruence
+      ; try match_destr
+      ; try intuition congruence.
+    Qed.
+
+    Lemma nnrs_imp_stmt_rename_nin s from to :
+      ~ In from (nnrs_imp_stmt_free_vars s) ->
+      nnrs_imp_stmt_rename s from to = s.
+    Proof.
+      induction s; simpl
+      ; repeat rewrite in_app_iff
+      ; repeat rewrite nnrs_imp_expr_rename_nin by tauto
+      ; intros
+      ; try congruence
+      ; repeat match_destr
+      ; repeat rewrite nnrs_imp_expr_rename_nin by tauto
+      ; try (intuition congruence)
+      ; try solve [rewrite IHs; intuition
+                   ; apply remove_nin_inv in H2; intuition]
+      ; try solve [rewrite IHs; intuition
+                   ; apply remove_nin_inv in H2; intuition].
+      - rewrite IHs2; intuition.
+        apply remove_nin_inv in H3; intuition.
+      - rewrite IHs1; intuition.
+        apply remove_nin_inv in H; intuition.
+      - rewrite IHs1, IHs2; intuition.
+        + apply remove_nin_inv in H3; intuition.
+        + apply remove_nin_inv in H; intuition.
+    Qed.
+    
+  End nfree.
+
+  Section involutive.
+
+    Lemma nnrs_imp_expr_rename_involutive e v v' :
+      ~ In v' (nnrs_imp_expr_free_vars e) ->
+      nnrs_imp_expr_rename (nnrs_imp_expr_rename e v v') v' v = e.
+    Proof.
+      induction e; simpl
+      ; repeat rewrite in_app_iff
+      ; intros inn
+      ; try rewrite IHe by tauto
+      ; try rewrite IHe1 by tauto
+      ; try rewrite IHe2 by tauto
+      ; try rewrite IHe3 by tauto
+      ; trivial.
+      - destruct (equiv_dec v0 v); match_destr; try congruence; tauto.
+    Qed.
+
+    Lemma nnrs_imp_stmt_rename_involutive s v v' :
+      ~ In v' (nnrs_imp_stmt_free_vars s) ->
+      ~ In v' (nnrs_imp_stmt_bound_vars s) ->
+      nnrs_imp_stmt_rename (nnrs_imp_stmt_rename s v v') v' v = s.
+    Proof.
+      induction s; simpl
+      ; repeat rewrite in_app_iff
+      ; intros innf innb
+      ; try rewrite nnrs_imp_expr_rename_involutive by tauto
+      ; try rewrite IHs by tauto
+      ; try rewrite IHs1 by tauto
+      ; try rewrite IHs2 by tauto
+      ; try rewrite IHs3 by tauto
+      ; trivial.
+      - destruct (equiv_dec v0 v); match_destr; unfold equiv, complement in *
+        ; try congruence.
+        tauto.
+      - f_equal.
+        + destruct o; trivial. rewrite nnrs_imp_expr_rename_involutive; tauto.
+        + intuition.
+          apply remove_nin_inv in H0; intuition.
+          destruct (equiv_dec v0 v'); try congruence.
+          match_destr.
+          rewrite nnrs_imp_stmt_rename_nin; tauto.
+      - f_equal.
+        intuition.
+        apply remove_nin_inv in H0; intuition.
+        destruct (equiv_dec v0 v'); try congruence.
+        match_destr.
+        rewrite nnrs_imp_stmt_rename_nin; tauto.
+      - intuition.
+        apply remove_nin_inv in H3.
+        apply remove_nin_inv in H4.
+        simpl in *.
+        intuition.
+        f_equal.
+        + destruct (equiv_dec v0 v'); try congruence.
+          match_destr.
+          rewrite nnrs_imp_stmt_rename_nin; tauto.
+        + destruct (equiv_dec v1 v'); try congruence.
+          match_destr.
+          rewrite nnrs_imp_stmt_rename_nin; tauto.
+    Qed.
+
+  End involutive.
+  
+  Section eval.
+
+    Lemma nnrs_imp_expr_eval_rename_in h c l σ e v v' d:
+      ~ In v (domain l) ->
+      ~ In v' (domain l) ->
+      ~ In v' (nnrs_imp_expr_free_vars e) ->
+      nnrs_imp_expr_eval h c (l++(v', d) :: σ) (nnrs_imp_expr_rename e v v')
+      = nnrs_imp_expr_eval h c (l++(v, d) :: σ) e.
+    Proof.
+      nnrs_imp_expr_cases (induction e) Case; simpl; trivial
+      ; repeat rewrite in_app_iff; intros
+      ; try solve [ rewrite IHe by intuition; trivial
+                  |  rewrite IHe1, IHe2 by intuition; trivial
+                  ].
+      - Case "NNRSimpVar"%string.
+        intuition.
+        repeat rewrite lookup_app.
+        destruct (equiv_dec v0 v); unfold equiv, complement in *
+        ; subst.
+        + repeat match_option
+          ; (try apply lookup_in_domain in eqq
+             ; try apply lookup_in_domain in eqq0; try contradiction).
+          simpl.
+          repeat match_destr; congruence.
+        + match_destr; simpl.
+          repeat match_destr; congruence.
+    Qed.
+    
+    Lemma nnrs_imp_expr_eval_rename h c σ e v v' d:
+      ~ In v' (nnrs_imp_expr_free_vars e) ->
+      nnrs_imp_expr_eval h c ((v', d) :: σ) (nnrs_imp_expr_rename e v v')
+      = nnrs_imp_expr_eval h c ((v, d) :: σ) e.
+    Proof.
+      apply (nnrs_imp_expr_eval_rename_in h c nil); simpl; tauto.
+    Qed.
+
+    Lemma nnrs_imp_stmt_eval_rename_in h c l σ s v v' d:
+      ~ In v (domain l) ->
+      ~ In v' (domain l) ->
+      ~ In v' (nnrs_imp_stmt_free_vars s) ->
+      ~ In v' (nnrs_imp_stmt_bound_vars s) ->
+
+      lift2P  (fun σ₁' σ₂' =>
+                 (forall l' d σ'',
+                     domain l' = domain l ->
+                     σ₁' = l' ++ (v',d)::σ'' ->
+                     σ₂' = l' ++ (v,d)::σ'')
+              )
+              (nnrs_imp_stmt_eval h c (nnrs_imp_stmt_rename s v v') (l++(v',d)::σ))
+              (nnrs_imp_stmt_eval h c s (l++(v,d)::σ)).
+    Proof.
+
+      Ltac disect_tac H stac
+        := 
+          unfold var in *
+          ; cut_to H; unfold domain in *; [ | solve[stac]..]
+          ; unfold lift2P in H
+          ; (repeat match_option_in H; try contradiction).
+
+      Ltac pcong
+        := solve[repeat (match goal with
+                         | [H: _ = _ |- _ ] => rewrite H in *; clear H
+                         end; try tauto)].
+
+      Ltac ren_eval_t stac
+        := repeat progress (
+                    repeat rewrite in_app_iff in *
+                    ; repeat
+                        match goal with
+                        | [H : ~ (_ \/ _ ) |- _ ] => apply not_or in H
+                        | [H : (_ \/ _ ) -> False |- _ ] => apply not_or in H
+                        | [H: _ /\ _ |- _ ] => destruct H
+                        | [ H : _ * _ |- _ ] => destruct H
+                        | [H: _::_ = _::_ |- _ ] => invcs H
+                        | [ H: domain (_ ++ _) = domain _ |- _ ] =>
+                          rewrite domain_app in H
+                          ; unfold domain in H
+                          ; symmetry in H; apply map_app_break in H
+                          ; destruct H as [? [?[?[??]]]]; subst; simpl in *
+                        | [ H: map (_ ++ _) = map _ |- _ ] =>
+                          rewrite map_app in H
+                          ; symmetry in H; apply map_app_break in H
+                          ; destruct H as [? [?[?[??]]]]; subst; simpl in *
+                        | [ H: _ :: _ = map _ ?x |- _ ] =>
+                          destruct x; try discriminate; simpl in H; invcs H
+                        | [ H: _ :: _ = domain ?x |- _ ] =>
+                          destruct x; try discriminate; simpl in H; invcs H
+                        | [H : ~ In _ (remove _ _ _) |- _ ] =>
+                          apply not_in_remove_impl_not_in in H; [| congruence]
+                        | [H : ?x ++ _ = ?y ++ _ |- _ ] =>
+                          let HH := fresh in
+                          assert (HH:domain y = domain x) by
+                              (unfold domain in *;
+                               try (intuition congruence)
+                               ; pcong)
+                          ; apply app_inv_head_domain in H;[clear HH|apply HH]
+                                                             
+
+                        | [ H: forall a b c, _ -> ?x1 ++ ?dd :: ?x2 = _ ++ _ :: _ -> _ |- _] =>
+                          specialize (H x1 (snd dd) x2); simpl in H
+                          ; match dd with
+                            | (_,_) => idtac
+                            | _ => destruct dd
+                            end
+                          ; simpl in *
+                          ; cut_to H; [ | eauto 3 | reflexivity]
+                        | [ H: forall a b c, _ -> ?dd0::?x1 ++ ?dd :: ?x2 = _ ++ _ :: _ -> _ |- _] =>
+                          specialize (H (dd0::x1) (snd dd) x2); simpl in H
+                          ; match dd with
+                            | (_,_) => idtac
+                            | _ => destruct dd
+                            end
+                          ; simpl in *
+                          ; cut_to H; [ | eauto 3 | reflexivity]
+
+                                        
+                        | [H : nnrs_imp_stmt_eval _ _ _ ?p1 = ?p2 |- _ ] =>
+                          match p1 with
+                          | p2 => fail 1
+                          | _ =>  extend (nnrs_imp_stmt_eval_domain_stack H); clear H
+                          end
+                            
+                        | [H:forall l σ d,
+                              _ -> _ -> _ -> _ -> lift2P _ (nnrs_imp_stmt_eval _ _ ?s _) _
+                                                         
+                              |- lift2P _ (olift _ (nnrs_imp_stmt_eval _ _ ?s (?l ++ (_, ?d) :: ?σ) ))
+                                        _ ] =>
+                          specialize (H l σ d)
+                          ; disect_tac H stac
+                        | [H:forall l σ d,
+                              _ -> _ -> _ -> _ -> lift2P _ (nnrs_imp_stmt_eval _ _ ?s _) _
+                                                         
+                              |- lift2P _ (nnrs_imp_stmt_eval _ _ ?s (?l ++ (_, ?d) :: ?σ) )
+                                        _ ] =>
+                          specialize (H l σ d)
+                          ; disect_tac H stac
+                        | [H:forall l σ d,
+                              _ -> _ -> _ -> _ -> lift2P _ (nnrs_imp_stmt_eval _ _ ?s _) _
+                                                         
+                              |- lift2P _ (match nnrs_imp_stmt_eval _ _ ?s (?x::?l ++ (_, ?d) :: ?σ)
+                                           with | Some _ => _ | None => _ end)
+                                        _ ] =>
+                          specialize (H (x::l) σ d); simpl in H
+                          ; disect_tac H stac
+                        end; simpl in *; trivial; intros; try subst; try solve [congruence | f_equal; congruence]).
+
+      Ltac ren_eval_tt := ren_eval_t ltac:(try tauto; try congruence).
+      
+      revert l σ d.
+      nnrs_imp_stmt_cases (induction s) Case; simpl; trivial
+      ; repeat rewrite in_app_iff in *; intros l σ d; intros
+      ; repeat rewrite nnrs_imp_expr_eval_rename_in by tauto
+      ; try solve [ rewrite IHs by intuition; trivial
+                  |  rewrite IHs1, IHs2 by intuition; trivial
+                  ].
+      - Case "NNRSimpSkip"%string.
+        ren_eval_tt.
+      - Case "NNRSimpSeq"%string.
+        ren_eval_tt.
+      - Case "NNRSimpAssign"%string.
+        match_destr; try reflexivity.
+        destruct (equiv_dec v0 v); unfold equiv, complement in *.
+        + subst.
+          repeat rewrite lookup_app.
+          rewrite (lookup_nin_none _ H0).
+          rewrite (lookup_nin_none _ H).
+          simpl.
+          repeat rewrite update_app_nin by trivial.
+          simpl.
+          destruct (string_dec v' v'); try congruence.
+          destruct (string_dec v v); try congruence.
+          ren_eval_tt.
+        + repeat rewrite lookup_app.
+          case_eq (lookup string_dec l v0); [intros ? inn | intros nin].
+          * repeat rewrite update_app_in
+              by (apply lookup_in_domain in inn; trivial).
+            simpl.
+            intros ? ? ? domeq eqq.
+            apply app_inv_head_domain in eqq
+            ; [ |rewrite domain_update_first; trivial].
+            destruct eqq as [eqq1 eqq2].
+            invcs eqq2.
+            trivial.
+          * apply lookup_none_nin in nin.
+            repeat rewrite update_app_nin by trivial.
+            simpl.
+            destruct (string_dec v0 v'); try tauto.
+            destruct (string_dec v0 v); try congruence.
+            match_destr; try reflexivity.
+            ren_eval_tt.
+      - Case "NNRSimpLet"%string.
+        destruct o.
+        + ren_eval_tt.
+          rewrite nnrs_imp_expr_eval_rename_in by trivial.
+          destruct (nnrs_imp_expr_eval h c (l ++ (v, d) :: σ) n); simpl; trivial.
+          destruct (equiv_dec v0 v); unfold equiv, complement in *.
+          * subst.
+            generalize (nnrs_imp_stmt_eval_unused h c
+                                                  ((v, Some d0) :: l) σ s v' d).
+            generalize (nnrs_imp_stmt_eval_unused h c
+                                                  ((v, Some d0) :: l) σ s v d).
+            simpl; intros HH1 HH2.
+            cut_to HH1; [| tauto].
+            cut_to HH2; [| tauto].
+            unfold lift2P in *.
+
+            repeat match_option_in HH1
+            ; rewrite eqq0 in *
+            ; repeat match_option_in HH2
+            ; subst
+            ; try contradiction
+            ; ren_eval_tt; subst
+            ; f_equal
+            ; unfold domain in *; eauto.
+          * ren_eval_tt.
+        + destruct (equiv_dec v0 v); unfold equiv, complement in *.
+          * subst.
+            generalize (nnrs_imp_stmt_eval_unused h c
+                                                  ((v, None) :: l) σ s v' d).
+            generalize (nnrs_imp_stmt_eval_unused h c
+                                                  ((v, None) :: l) σ s v d).
+            simpl; intros HH1 HH2.
+            cut_to HH1; [| tauto].
+            simpl in H1.
+            apply remove_nin_inv in H1.
+            cut_to HH2; [ | intuition ].
+            unfold lift2P in *.
+
+            repeat match_option_in HH1
+            ; rewrite eqq0 in *
+            ; repeat match_option_in HH2
+            ; subst
+            ; try contradiction
+            ; ren_eval_tt; subst
+            ; f_equal
+            ; unfold domain in *; eauto.
+          * ren_eval_tt.
+      - Case "NNRSimpFor"%string.
+        ren_eval_tt.
+        rewrite nnrs_imp_expr_eval_rename_in by trivial.
+        destruct (nnrs_imp_expr_eval h c (l ++ (v, d) :: σ) n); simpl; trivial.
+        destruct d0; simpl; trivial.
+        revert l σ d H H0.
+        induction l0; intros l σ d ninv ninv'; simpl; ren_eval_tt.
+        destruct (equiv_dec v0 v); unfold equiv, complement in *.
+        + subst.
+          generalize (nnrs_imp_stmt_eval_unused h c
+                                                ((v, Some a) :: l) σ s v' d).
+          generalize (nnrs_imp_stmt_eval_unused h c
+                                                ((v, Some a) :: l) σ s v d).
+          simpl; intros HH1 HH2.
+          cut_to HH1; [| tauto].
+          simpl in H1.
+          cut_to HH2; [ | intuition ].
+          unfold lift2P in *.
+          
+          repeat match_option_in HH1
+          ; rewrite eqq0 in *
+          ; repeat match_option_in HH2
+          ; subst
+          ; try contradiction
+          ; ren_eval_tt; subst
+          ; f_equal
+          ; unfold domain in *; eauto.
+          * specialize (IHl0 x x0 o0).
+            unfold var in *.
+            { cut_to IHl0.
+              - unfold lift2P in *.
+                repeat match_option_in IHl0.
+                ren_eval_tt.
+              - pcong.
+              - pcong.
+            }
+        + specialize (IHs ((v0, Some a)::l) σ d); simpl in IHs.
+          cut_to IHs; simpl; [ | intuition..].
+          unfold lift2P in *.
+          unfold var in *.
+          repeat match_option_in IHs
+          ; try contradiction
+          ; ren_eval_tt.
+          * specialize (IHl0 x x0 o0).
+            { cut_to IHl0.
+              - unfold lift2P in *.
+                repeat match_option_in IHl0.
+                ren_eval_tt.
+                pcong.
+              - unfold domain in *; congruence.
+              - unfold domain in *; congruence.
+            }
+          * f_equal.
+            unfold domain in *; congruence.
+      - Case "NNRSimpIf"%string.
+        ren_eval_tt.
+        rewrite nnrs_imp_expr_eval_rename_in by trivial.
+        destruct (nnrs_imp_expr_eval h c (l ++ (v, d) :: σ) n); simpl; trivial.
+        destruct d0; simpl; trivial. 
+        destruct b; ren_eval_tt.
+      - Case "NNRSimpEither"%string.
+        ren_eval_tt.
+        rewrite nnrs_imp_expr_eval_rename_in by trivial.
+        destruct (nnrs_imp_expr_eval h c (l ++ (v, d) :: σ) n); simpl; trivial.
+        destruct d0; simpl; trivial.
+        + destruct (equiv_dec v0 v); unfold equiv, complement in *.
+          * subst.
+            generalize (nnrs_imp_stmt_eval_unused h c
+                                                  ((v, Some d0) :: l) σ s1 v' d).
+            generalize (nnrs_imp_stmt_eval_unused h c
+                                                  ((v, Some d0) :: l) σ s1 v d).
+            simpl; intros HH1 HH2.
+            cut_to HH1; [| tauto].
+            simpl in H1.
+            cut_to HH2; [ | intuition ].
+            unfold lift2P in *.
+
+            repeat match_option_in HH1
+            ; rewrite eqq0 in *
+            ; repeat match_option_in HH2
+            ; subst
+            ; try contradiction
+            ; ren_eval_tt; subst
+            ; f_equal
+            ; unfold domain in *; eauto.
+          * ren_eval_tt. 
+        + destruct (equiv_dec v1 v); unfold equiv, complement in *.
+          * subst.
+            generalize (nnrs_imp_stmt_eval_unused h c
+                                                  ((v, Some d0) :: l) σ s2 v' d).
+            generalize (nnrs_imp_stmt_eval_unused h c
+                                                  ((v, Some d0) :: l) σ s2 v d).
+            simpl; intros HH1 HH2.
+            cut_to HH1; [| tauto].
+            simpl in H1.
+            cut_to HH2; [ | intuition ].
+            unfold lift2P in *.
+
+            repeat match_option_in HH1
+            ; rewrite eqq0 in *
+            ; repeat match_option_in HH2
+            ; subst
+            ; try contradiction
+            ; ren_eval_tt; subst
+            ; f_equal
+            ; unfold domain in *; eauto.
+          * ren_eval_tt. 
+    Qed.                               
+
+    Lemma nnrs_imp_stmt_eval_rename h c σ s v v' d:
+      ~ In v' (nnrs_imp_stmt_free_vars s) ->
+      ~ In v' (nnrs_imp_stmt_bound_vars s) ->
+      match
+        (nnrs_imp_stmt_eval h c (nnrs_imp_stmt_rename s v v') ((v',d)::σ)),
+        (nnrs_imp_stmt_eval h c s ((v,d)::σ)) with
+      | None, None => True
+      | Some ((v₁,d₁)::σ₁'), Some ((v₂,d₂)::σ₂') => v₁ = v' /\ v₂ = v /\ d₁ = d₂ /\ σ₁' = σ₂'
+      | _, _ => False
+      end.
+    Proof.
+      intros inn.
+      generalize (nnrs_imp_stmt_eval_rename_in h c nil σ s v v' d)
+      ; simpl; intros; intuition.
+      match_option
+      ; rewrite eqq in *
+      ; simpl in *
+      ; trivial.
+      match_option_in H; try contradiction.
+      apply nnrs_imp_stmt_eval_domain_stack in eqq.
+      apply nnrs_imp_stmt_eval_domain_stack in eqq0.
+      simpl in *.
+      destruct p; simpl in *; invcs eqq.
+      destruct p0; simpl in *; invcs eqq0.
+      destruct p; destruct p0; simpl.
+      specialize (H nil o p1 (eq_refl _) (eq_refl _))
+      ; simpl in *.
+      invcs H.
+      tauto.
+    Qed.
+    
+  End eval.
+
+  Section core.
+
+    Lemma nnrs_imp_expr_rename_core e v v' :
+      nnrs_imp_exprIsCore (nnrs_imp_expr_rename e v v') <->
+      nnrs_imp_exprIsCore e.
+    Proof.
+      induction e; simpl; intuition.
+    Qed.
+
+    Lemma nnrs_imp_stmt_rename_core_f s v v' :
+      nnrs_imp_stmtIsCore s ->
+      nnrs_imp_stmtIsCore (nnrs_imp_stmt_rename s v v').
+    Proof.
+      induction s; simpl
+      ; repeat rewrite nnrs_imp_expr_rename_core in *
+      ; intuition.
+      - destruct o; match_destr
+        ; repeat rewrite nnrs_imp_expr_rename_core in *
+        ; intuition.
+      - match_destr
+        ; repeat rewrite nnrs_imp_expr_rename_core in *
+        ; intuition.
+      - match_destr 
+        ; repeat rewrite nnrs_imp_expr_rename_core in *
+        ; intuition.
+      - match_destr
+        ; repeat rewrite nnrs_imp_expr_rename_core in *
+        ; intuition.
+    Qed.
+
+    Lemma nnrs_imp_stmt_rename_core_b s v v' :
+      nnrs_imp_stmtIsCore (nnrs_imp_stmt_rename s v v') ->
+      nnrs_imp_stmtIsCore s.
+    Proof.
+      induction s; simpl
+      ; repeat rewrite nnrs_imp_expr_rename_core in *
+      ; intuition.
+      - destruct o; match_destr_in H
+        ; repeat rewrite nnrs_imp_expr_rename_core in *
+        ; intuition.
+      - match_destr_in H1
+        ; repeat rewrite nnrs_imp_expr_rename_core in *
+        ; intuition.
+      - match_destr_in H
+        ; repeat rewrite nnrs_imp_expr_rename_core in *
+        ; intuition.
+      - match_destr_in H2
+        ; repeat rewrite nnrs_imp_expr_rename_core in *
+        ; intuition.
+    Qed.
+
+    Lemma nnrs_imp_stmt_rename_core s v v' :
+      nnrs_imp_stmtIsCore (nnrs_imp_stmt_rename s v v') <->
+      nnrs_imp_stmtIsCore s.
+    Proof.
+      split; intros HH.
+      - eapply nnrs_imp_stmt_rename_core_b; eauto.
+      - eapply nnrs_imp_stmt_rename_core_f; eauto.
+    Qed.
+    
+  End core.
+
+End NNRSimpRename.
