coq/NNRSimp/Typing/TNNRSimpRename.v
@@ -1,0 +1,428 @@
+(*
+ * Copyright 2015-2016 IBM Corporation
+ *
+ * Licensed under the Apache License, Version 2.0 (the "License");
+ * you may not use this file except in compliance with the License.
+ * You may obtain a copy of the License at
+ *
+ * http://www.apache.org/licenses/LICENSE-2.0
+ *
+ * Unless required by applicable law or agreed to in writing, software
+ * distributed under the License is distributed on an "AS IS" BASIS,
+ * WITHOUT WARRANTIES OR CONDITIONS OF ANY KIND, either express or implied.
+ * See the License for the specific language governing permissions and
+ * limitations under the License.
+ *)
+
+Require Import String.
+Require Import List.
+Require Import Arith.
+Require Import EquivDec.
+Require Import Morphisms.
+Require Import Arith.
+Require Import Max.
+Require Import Bool.
+Require Import Peano_dec.
+Require Import EquivDec.
+Require Import Decidable.
+Require Import Utils.
+Require Import CommonSystem.
+Require Import NNRSimp.
+Require Import NNRSimpVars.
+Require Import NNRSimpUsage.
+Require Import NNRSimpRename.
+Require Import TNNRSimp.
+
+Section TNNRSimpRename.
+  Local Open Scope nnrs_imp.
+
+  Context {m:basic_model}.
+
+  Hint Constructors nnrs_imp_expr_type.
+  Hint Constructors nnrs_imp_stmt_type.
+
+  Lemma nnrs_imp_expr_type_rename_in_f Γc l Γ e (v v':var) τ (τo:rtype) :
+    ~ In v (domain l) ->
+    ~ In v' (domain l) ->
+    ~ In v' (nnrs_imp_expr_free_vars e) ->
+    [ Γc ; (l++(v,τ)::Γ)  ⊢ e ▷ τo ] ->
+    [ Γc ; (l++(v',τ)::Γ)  ⊢ nnrs_imp_expr_rename e v v' ▷ τo ]%nnrs_imp_scope.
+  Proof.
+    revert τo.
+    nnrs_imp_expr_cases (induction e) Case; simpl; trivial
+    ; intros τo ??? typ
+    ; invcs typ
+    ; repeat rewrite in_app_iff in *
+    ; eauto 3.
+    -  Case "NNRSimpVar"%string.
+       econstructor.
+       repeat rewrite lookup_app in *.
+       destruct (equiv_dec v0 v); unfold equiv, complement in *
+       ; subst.
+       + repeat match_option
+         ; try solve [(try apply lookup_in_domain in eqq
+                       ; try apply lookup_in_domain in eqq0; try contradiction)].
+         repeat match_option_in H4
+         ; try solve [(try apply lookup_in_domain in eqq
+                       ; try apply lookup_in_domain in eqq0; try contradiction)].
+         simpl in *.
+         match_destr_in H4; try congruence.
+         match_destr; try congruence.
+       + match_option; simpl.
+         * rewrite eqq in H4; trivial.
+         * rewrite eqq in H4; simpl in *.
+           match_destr_in H4; try congruence.
+           match_destr; try congruence.
+           intuition.
+    - Case "NNRSimpBinop"%string.
+      econstructor; eauto.
+  Qed.
+
+  Lemma nnrs_imp_expr_type_rename_f Γc Γ e (v v':var) τ (τo:rtype) :
+    ~ In v' (nnrs_imp_expr_free_vars e) ->
+    [ Γc ; ((v,τ)::Γ)  ⊢ e ▷ τo ] ->
+    [ Γc ; ((v',τ)::Γ)  ⊢ nnrs_imp_expr_rename e v v' ▷ τo ]%nnrs_imp_scope.
+  Proof.
+    intros.
+    apply (nnrs_imp_expr_type_rename_in_f Γc nil Γ); simpl; tauto.
+  Qed.
+
+  Lemma nnrs_imp_stmt_type_rename_in_f Γc l Γ s (v v':var) τ :
+    ~ In v (domain l) ->
+    ~ In v' (domain l) ->
+    ~ In v' (nnrs_imp_stmt_free_vars s) ->
+    ~ In v' (nnrs_imp_stmt_bound_vars s) ->
+    [ Γc ; (l++(v,τ)::Γ)   ⊢ s ] ->
+    [ Γc ; (l++(v',τ)::Γ) ⊢ nnrs_imp_stmt_rename s v v' ].
+  Proof.
+    Hint Resolve nnrs_imp_expr_type_rename_in_f.
+
+    revert l Γ τ
+    ; nnrs_imp_stmt_cases (induction s) Case
+    ; simpl; intros l Γ τ ninl ninl' nine ninb typ
+    ; repeat rewrite in_app_iff in nine
+    ; repeat rewrite in_app_iff in ninb
+    ; invcs typ.
+    - Case "NNRSimpSkip"%string.
+      eauto.
+    - Case "NNRSimpSeq"%string.
+      intuition eauto.
+    - Case "NNRSimpAssign"%string.
+      match_destr; unfold equiv, complement in *.
+      + subst.
+        econstructor; eauto.
+        repeat rewrite lookup_app in *.
+        repeat rewrite lookup_nin_none in * by trivial.
+        simpl in *.
+        match_destr_in H3; try contradiction.
+        match_destr; try contradiction.
+      + econstructor; eauto.
+        repeat rewrite lookup_app in *.
+        simpl in *.
+        match_destr_in H3; try contradiction.
+        match_destr_in H3; try contradiction.
+        match_destr; try tauto.
+    - Case "NNRSimpLet"%string.
+      match_destr; unfold equiv, complement in *.
+      + subst.
+        econstructor; eauto.
+        apply (nnrs_imp_stmt_type_unused_remove Γc ((v,τ0)::l)) in H4
+        ; simpl; try tauto.
+        apply (nnrs_imp_stmt_type_unused_add Γc ((v, τ0)::l))
+        ; simpl; trivial.
+        intuition.
+        destruct (remove_nin_inv H3); eauto.
+      + econstructor; eauto.
+        specialize (IHs ((v0, τ0) :: l)); simpl in IHs.
+        eapply IHs; eauto
+        ; intuition.
+        destruct (remove_nin_inv H1); eauto.
+    - Case "NNRSimpLet"%string.
+      match_destr; unfold equiv, complement in *.
+      + subst.
+        econstructor; eauto.
+        apply (nnrs_imp_stmt_type_unused_remove Γc ((v,τ0)::l)) in H4
+        ; simpl; try tauto.
+        apply (nnrs_imp_stmt_type_unused_add Γc ((v, τ0)::l))
+        ; simpl; trivial.
+        intuition.
+        destruct (remove_nin_inv H3); eauto.
+      + econstructor; eauto.
+        * rewrite nnrs_imp_stmt_rename_var_usage_neq; tauto.
+        * specialize (IHs ((v0, τ0) :: l)); simpl in IHs.
+          eapply IHs; eauto
+          ; intuition.
+          destruct (remove_nin_inv H1); eauto.
+    - Case "NNRSimpFor"%string.
+      match_destr; unfold equiv, complement in *.
+      + subst.
+        econstructor; eauto.
+        apply (nnrs_imp_stmt_type_unused_remove Γc ((v,τ0)::l)) in H4
+        ; simpl; try tauto.
+        apply (nnrs_imp_stmt_type_unused_add Γc ((v, τ0)::l))
+        ; simpl; trivial.
+        intuition.
+        destruct (remove_nin_inv H3); eauto.
+      + econstructor; eauto.
+        specialize (IHs ((v0, τ0) :: l)); simpl in IHs.
+        eapply IHs; eauto
+        ; intuition.
+        destruct (remove_nin_inv H1); eauto.
+    - Case "NNRSimpIf"%string.
+      econstructor; intuition eauto.
+    - Case "NNRSimpEither"%string.
+      econstructor; eauto.
+      + match_destr; unfold equiv, complement in *.
+        * subst.
+          apply (nnrs_imp_stmt_type_unused_remove Γc ((v,τl)::l)) in H6
+          ; simpl; try tauto.
+          apply (nnrs_imp_stmt_type_unused_add Γc ((v,τl)::l))
+          ; simpl; trivial.
+          intuition.
+          destruct (remove_nin_inv H0); eauto.
+        * specialize (IHs1 ((v0, τl) :: l)); simpl in IHs1.
+          eapply IHs1; eauto
+          ; intuition.
+          destruct (remove_nin_inv H5); eauto.
+      + match_destr; unfold equiv, complement in *.
+        * subst.
+          apply (nnrs_imp_stmt_type_unused_remove Γc ((v,τr)::l)) in H7
+          ; simpl; try tauto.
+          apply (nnrs_imp_stmt_type_unused_add Γc ((v,τr)::l))
+          ; simpl; trivial.
+          intuition.
+          destruct (remove_nin_inv H8); eauto.
+        * specialize (IHs2 ((v1, τr) :: l)); simpl in IHs2.
+          eapply IHs2; simpl in *; eauto
+          ; intuition.
+          destruct (remove_nin_inv H8); eauto.
+  Qed.
+
+  Lemma nnrs_imp_stmt_type_rename_f Γc Γ s (v v':var) τ :
+    ~ In v' (nnrs_imp_stmt_free_vars s) ->
+    ~ In v' (nnrs_imp_stmt_bound_vars s) ->
+    [ Γc ; ((v,τ)::Γ)   ⊢ s ] ->
+    [ Γc ; ((v',τ)::Γ) ⊢ nnrs_imp_stmt_rename s v v' ].
+  Proof.
+    intros.
+    apply (nnrs_imp_stmt_type_rename_in_f Γc nil); tauto.
+  Qed.
+  
+  Lemma nnrs_imp_expr_type_rename_in_b Γc l Γ e (v v':var) τ (τo:rtype) :
+    ~ In v (domain l) ->
+    ~ In v' (domain l) ->
+    ~ In v' (nnrs_imp_expr_free_vars e) ->
+    [ Γc ; (l++(v',τ)::Γ)  ⊢ nnrs_imp_expr_rename e v v' ▷ τo ]%nnrs_imp_scope ->
+    [ Γc ; (l++(v,τ)::Γ)  ⊢ e ▷ τo ].
+  Proof.
+    revert τo.
+    nnrs_imp_expr_cases (induction e) Case; simpl; trivial
+    ; intros τo ??? typ
+    ; invcs typ
+    ; repeat rewrite in_app_iff in *
+    ; eauto 3.
+    - Case "NNRSimpVar"%string.
+      econstructor.
+      repeat rewrite lookup_app in *.
+      destruct (equiv_dec v0 v); unfold equiv, complement in *
+      ; subst; simpl in *.
+      + repeat match_option
+        ; try solve [(try apply lookup_in_domain in eqq
+                      ; try apply lookup_in_domain in eqq0; try contradiction)].
+        repeat match_option_in H4
+        ; try solve [(try apply lookup_in_domain in eqq
+                      ; try apply lookup_in_domain in eqq0; try contradiction)].
+        simpl in *.
+        match_destr_in H4; try congruence.
+        match_destr; try congruence.
+      + match_option; simpl.
+        * rewrite eqq in H4; trivial.
+        * rewrite eqq in H4; simpl in *.
+          match_destr; try congruence.
+          match_destr_in H4; try congruence.
+          intuition.
+    - Case "NNRSimpBinop"%string.
+      econstructor; eauto.
+  Qed.
+
+  Lemma nnrs_imp_expr_type_rename_b Γc Γ e (v v':var) τ (τo:rtype) :
+    ~ In v' (nnrs_imp_expr_free_vars e) ->
+    [ Γc ; ((v',τ)::Γ)  ⊢ nnrs_imp_expr_rename e v v' ▷ τo ]%nnrs_imp_scope ->
+    [ Γc ; ((v,τ)::Γ)  ⊢ e ▷ τo ].
+  Proof.
+    intros.
+    eapply (nnrs_imp_expr_type_rename_in_b Γc nil Γ); eauto; tauto.
+  Qed.
+
+  Lemma nnrs_imp_stmt_type_rename_in_b Γc l Γ s (v v':var) τ :
+    ~ In v (domain l) ->
+    ~ In v' (domain l) ->
+    ~ In v' (nnrs_imp_stmt_free_vars s) ->
+    ~ In v' (nnrs_imp_stmt_bound_vars s) ->
+    [ Γc ; (l++(v',τ)::Γ) ⊢ nnrs_imp_stmt_rename s v v' ] ->
+    [ Γc ; (l++(v,τ)::Γ)   ⊢ s ].
+  Proof.
+    Hint Resolve nnrs_imp_expr_type_rename_in_b.
+
+    revert l Γ τ
+    ; nnrs_imp_stmt_cases (induction s) Case
+    ; simpl; intros l Γ τ ninl ninl' nine ninb typ
+    ; repeat rewrite in_app_iff in nine
+    ; repeat rewrite in_app_iff in ninb
+    ; invcs typ.
+    - Case "NNRSimpSkip"%string.
+      eauto.
+    - Case "NNRSimpSeq"%string.
+      intuition eauto.
+    - Case "NNRSimpAssign"%string.
+      match_destr_in H3; unfold equiv, complement in *.
+      + subst.
+        econstructor; eauto.
+        repeat rewrite lookup_app in *.
+        repeat rewrite lookup_nin_none in * by trivial.
+        simpl in *.
+        match_destr_in H3; try contradiction.
+        invcs H3.
+        match_destr; try contradiction.
+      + econstructor; eauto.
+        repeat rewrite lookup_app in *.
+        simpl in *.
+        match_destr_in H3; try contradiction.
+        match_destr; try tauto.
+        match_destr_in H3; try contradiction.
+        tauto.
+    - Case "NNRSimpLet"%string.
+      destruct o; try discriminate.
+      invcs H0.
+      econstructor; eauto.
+      match_destr_in H4; unfold equiv, complement in *.
+      + subst.
+        apply (nnrs_imp_stmt_type_unused_add Γc ((v, τ0)::l))
+        ; simpl; try tauto.
+        apply (nnrs_imp_stmt_type_unused_remove Γc ((v,τ0)::l)) in H4
+        ; simpl; try tauto.
+        intuition.
+        destruct (remove_nin_inv H3); eauto.
+      + specialize (IHs ((v0, τ0) :: l)); simpl in IHs.
+        eapply IHs; eauto
+        ; intuition.
+        destruct (remove_nin_inv H1); eauto.
+    - Case "NNRSimpLet"%string.
+      destruct o; try discriminate.
+      match_destr_in H4; unfold equiv, complement in *.
+      + subst.
+        econstructor; eauto.
+        apply (nnrs_imp_stmt_type_unused_add Γc ((v, τ0)::l))
+        ; simpl; try tauto.
+        apply (nnrs_imp_stmt_type_unused_remove Γc ((v,τ0)::l)) in H4
+        ; simpl; try tauto.
+        intuition.
+        destruct (remove_nin_inv H5); eauto.
+      + econstructor; eauto.
+        * rewrite nnrs_imp_stmt_rename_var_usage_neq in H2; tauto.
+        * specialize (IHs ((v0, τ0) :: l)); simpl in IHs.
+          eapply IHs; eauto
+          ; intuition.
+          destruct (remove_nin_inv H3); eauto.
+    - Case "NNRSimpFor"%string.
+      match_destr_in H4; unfold equiv, complement in *.
+      + subst.
+        econstructor; eauto.
+        apply (nnrs_imp_stmt_type_unused_add Γc ((v, τ0)::l))
+        ; simpl; try tauto.
+        apply (nnrs_imp_stmt_type_unused_remove Γc ((v,τ0)::l)) in H4
+        ; simpl; try tauto.
+        intuition.
+        destruct (remove_nin_inv H3); eauto.
+      + econstructor; eauto.
+        specialize (IHs ((v0, τ0) :: l)); simpl in IHs.
+        eapply IHs; eauto
+        ; intuition.
+        destruct (remove_nin_inv H1); eauto.
+    - Case "NNRSimpIf"%string.
+      econstructor; intuition eauto.
+    - Case "NNRSimpEither"%string.
+      econstructor; eauto.
+      + match_destr_in H6; unfold equiv, complement in *.
+        * subst.
+          apply (nnrs_imp_stmt_type_unused_add Γc ((v,τl)::l))
+          ; simpl; try tauto.
+          apply (nnrs_imp_stmt_type_unused_remove Γc ((v,τl)::l)) in H6
+          ; simpl; try tauto.
+          intuition.
+          destruct (remove_nin_inv H0); eauto.
+        * specialize (IHs1 ((v0, τl) :: l)); simpl in IHs1.
+          eapply IHs1; eauto
+          ; intuition.
+          destruct (remove_nin_inv H5); eauto.
+      + match_destr_in H7; unfold equiv, complement in *.
+        * subst.
+          apply (nnrs_imp_stmt_type_unused_add Γc ((v,τr)::l))
+          ; simpl; try tauto.
+          apply (nnrs_imp_stmt_type_unused_remove Γc ((v,τr)::l)) in H7
+          ; simpl; try tauto.
+          intuition.
+          destruct (remove_nin_inv H8); eauto.
+        * specialize (IHs2 ((v1, τr) :: l)); simpl in IHs2.
+          eapply IHs2; simpl in *; eauto
+          ; intuition.
+          destruct (remove_nin_inv H8); eauto.
+  Qed.
+
+  Lemma nnrs_imp_stmt_type_rename_b Γc Γ s (v v':var) τ :
+    ~ In v' (nnrs_imp_stmt_free_vars s) ->
+    ~ In v' (nnrs_imp_stmt_bound_vars s) ->
+    [ Γc ; ((v',τ)::Γ) ⊢ nnrs_imp_stmt_rename s v v' ] ->
+    [ Γc ; ((v,τ)::Γ)   ⊢ s ].
+  Proof.
+    intros.
+    eapply (nnrs_imp_stmt_type_rename_in_b Γc nil); eauto.
+  Qed.
+
+  Theorem nnrs_imp_expr_type_rename_in Γc l Γ e (v v':var) τ (τo:rtype) :
+    ~ In v (domain l) ->
+    ~ In v' (domain l) ->
+    ~ In v' (nnrs_imp_expr_free_vars e) ->
+    [ Γc ; (l++(v',τ)::Γ)  ⊢ nnrs_imp_expr_rename e v v' ▷ τo ]%nnrs_imp_scope <->
+    [ Γc ; (l++(v,τ)::Γ)  ⊢ e ▷ τo ].
+  Proof.
+    intros; split; intros.
+    - eapply nnrs_imp_expr_type_rename_in_b; eauto.
+    - eapply nnrs_imp_expr_type_rename_in_f; eauto.
+  Qed.
+
+  Corollary nnrs_imp_expr_type_rename Γc Γ e (v v':var) τ (τo:rtype) :
+    ~ In v' (nnrs_imp_expr_free_vars e) ->
+    [ Γc ; ((v',τ)::Γ)  ⊢ nnrs_imp_expr_rename e v v' ▷ τo ]%nnrs_imp_scope <->
+    [ Γc ; ((v,τ)::Γ)  ⊢ e ▷ τo ].
+  Proof.
+    intros; split; intros.
+    - eapply nnrs_imp_expr_type_rename_b; eauto.
+    - eapply nnrs_imp_expr_type_rename_f; eauto.
+  Qed.
+
+  Theorem nnrs_imp_stmt_type_rename_in Γc l Γ s (v v':var) τ :
+    ~ In v (domain l) ->
+    ~ In v' (domain l) ->
+    ~ In v' (nnrs_imp_stmt_free_vars s) ->
+    ~ In v' (nnrs_imp_stmt_bound_vars s) ->
+    [ Γc ; (l++(v',τ)::Γ) ⊢ nnrs_imp_stmt_rename s v v' ] <->
+    [ Γc ; (l++(v,τ)::Γ)   ⊢ s ].
+  Proof.
+    intros; split; intros.
+    - eapply nnrs_imp_stmt_type_rename_in_b; eauto.
+    - eapply nnrs_imp_stmt_type_rename_in_f; eauto.
+  Qed.
+
+  Corollary nnrs_imp_stmt_type_rename Γc Γ s (v v':var) τ :
+    ~ In v' (nnrs_imp_stmt_free_vars s) ->
+    ~ In v' (nnrs_imp_stmt_bound_vars s) ->
+    [ Γc ; ((v',τ)::Γ) ⊢ nnrs_imp_stmt_rename s v v' ] <->
+    [ Γc ; ((v,τ)::Γ)   ⊢ s ].
+  Proof.
+    intros; split; intros.
+    - eapply nnrs_imp_stmt_type_rename_b; eauto.
+    - eapply nnrs_imp_stmt_type_rename_f; eauto.
+  Qed.
+  
+End TNNRSimpRename.
